finished edge coloring library

Vizing/new/EdgeColoring.lean
@@ -1,566 +1,282 @@
 import Vizing.new.Graph
-import Mathlib.Tactic
-import Mathlib.Data.List.Lemmas
-import Mathlib.Data.Finset.Card
+import Vizing.new.SetSet
+import Vizing.new.Nbhd
 
 set_option linter.dupNamespace false
+set_option push_neg.use_distrib true
+-- set_option trace.profiler true
 
 namespace EdgeColoring
 open Graph
+open SetSet
+open Nbhd
 
 /-
 Implementation of a basic edge-coloring library,
 where `EdgeColoring c` represents a c-edge-coloring of a graph on [n] vertices.
 -/
 
-variable (c : Nat) (n : Nat) (G : Graph n)
-abbrev Color := Option (Fin c)
-
-def coloringSizeAx (C : Array (Array (Color c))) :=
-  C.size = n ∧ ∀ x ∈ C, x.size = n
-
-abbrev Mat := {C : Array (Array (Color c)) // coloringSizeAx c n C}
-
-def set_set (M : Mat c n) (a : Color c)
-  (i j : Fin n) : Mat c n :=
-  have ⟨M, ⟨h1, h2⟩⟩ := M
-  let M' := M.set i (M[i].set j a (by simp_all)) (by simp_all)
-  have h : coloringSizeAx c n M' := by
-    simp_all [coloringSizeAx, M']
-    intro x h
-    rcases (Array.mem_or_eq_of_mem_set h) with (this | this)
-    · simp_all only [M']
-    · rw [this]
-      simp_all [Array.size_set]
-  ⟨M', h⟩
-
-theorem set_set_spec (M : Mat c n) (a : Color c) (i j : Fin n) :
-  have ⟨N, ⟨hn1, hn2⟩⟩ := set_set c n M a i j
-  have ⟨M, ⟨hm1, hm2⟩⟩ := M
-  ∀ u v : Fin n,
-    (M[u]'(by simp_all))[v]'(by simp_all) = (N[u]'(by simp_all))[v]'(by simp_all) ∨
-    (N[u]'(by simp_all))[v]'(by simp_all) = a ∧ i = u ∧ j = v := by
-    simp_all; repeat split
-    rename_i _ N hn1 hn2 _ M hm1 hm2 N_def
-    intro u v
-    unfold set_set at N_def; simp at N_def; subst N_def
-    by_cases h : i = u ∧ j = v
-    · right
-      constructor
-      · rcases h with ⟨hl, hr⟩
-        rw [← hl, ← hr]
-        simp_all
-      · exact h
-    · left
-      by_cases h' : i = u
-      · simp_all
-        exact Eq.symm (@Array.getElem_set_ne _ M[u] j
-        (by simp_all) a v (by simp_all) (by exact Fin.val_ne_of_ne h))
-      · have := @Array.getElem_set_ne _ M i (by simp_all)
-          (M[i].set j a (by simp_all)) u (by simp_all) (by exact Fin.val_ne_of_ne h')
-        simp_all
-
-def coloringRepresentsEdgesAx (C : Mat c n) (G : Graph n) :=
-  have aux1 : ∀ e : Edge n, e.1 < C.val.size := by
-    intro e
-    linarith [(e.1).isLt, C.prop.left]
-  have aux2 : ∀ e : Edge n, e.2 < (C.val[e.1]'(aux1 e)).size := by
-    intro e
-    have h1 := C.prop.right (C.val[e.1]'(aux1 e))
-    have h2 := (e.2).isLt
-    simp at h1
-    exact Nat.lt_of_lt_of_eq h2 (Eq.symm h1)
-  let E := toEdgeSet n G
-  ∀ e : Edge n, ((C.val[e.1]'(aux1 e))[e.2]'(aux2 e)).isSome → present n G e
-
-def coloringValidAx (C : Mat c n) :=
-  have aux : ∀ v : Vertex n, v < C.val.size := by
-    intro v
-    linarith [v.isLt, C.prop.left]
-  ∀ v : Vertex n, (List.filterMap id (C.val[v]'(aux v)).toList).Nodup
-
-def coloringSymmAx (C : Mat c n) :=
-  have ⟨C, ⟨h1, h2⟩⟩ := C
-  ∀ u v : Fin n, (C[u]'(by simp_all))[v]'(by simp_all) = (C[v]'(by simp_all))[u]'(by simp_all)
-
-abbrev EdgeColoring := {C : Mat c n // coloringRepresentsEdgesAx c n C G ∧ coloringValidAx c n C ∧ coloringSymmAx c n C}
-
-variable (C : EdgeColoring c n G)
-@[simp]
-theorem edgesInRange (e : Edge n) :
-  e.1 < C.val.val.size ∧
-  e.2 < (C.val.val[e.1]'(by simp_all only [Fin.is_lt, C.val.prop.left])).size := by
-    have ⟨⟨C, ⟨h1, h2⟩⟩, h3⟩ := C
-    constructor
-    all_goals simp_all
-
-theorem verticesInRange (v : Vertex n) :
-  v < C.val.val.size := by
-  have ⟨⟨C, ⟨h1, _⟩⟩, _⟩ := C
-  simp_all
-
-def color (e : Edge n) : Color c :=
-  have ⟨aux1, aux2⟩ := edgesInRange c n G C e
-  C.val.val[e.1][e.2]
-
-def coloredNbors (v : Vertex n) : Nbors n :=
-  have aux1 := verticesInRange c n G C v
-  have ⟨⟨C, ⟨h1, h2⟩⟩, ⟨h3, h4⟩⟩ := C
-  have := G.prop.right
-  have aux2 : C[v].size = n := by
-    simp_all
-  have aux3 : ∀ x : Vertex n, x < C[v].size := by
-    simp_all
-  let N := (List.finRange n).filter (fun x => (C[v][x]'(aux3 x)).isSome)
-  have ax1 : nborsSizeAx n N := by
-    have h4: v ∉ N := by
-      specialize h3 (v, v)
-      simp_all [N]
-      contrapose! h3
-      constructor
-      · exact Option.isSome_iff_ne_none.mpr h3
-      · have := G.prop.right v
-        simp_all [present, nbhd]
-    have h5 : N.length ≤ (List.finRange n).length := by
-      apply List.length_filter_le
-    rcases lt_or_eq_of_le h5 with (h5 | h5)
-    · simp_all; assumption
-    · unfold N at h4 h5
-      apply List.length_filter_eq_length_iff.mp at h5
-      specialize h5 v (by exact List.mem_finRange v)
-      simp_all
-  have ax2 : nborsRepeatsAx n N := by
-    apply List.Nodup.filter
-    exact List.nodup_finRange n
-  ⟨N, ⟨ax1, ax2⟩⟩
-
-def incidentColorsOn (v : Vertex n) :=
-  have := verticesInRange c n G C v
-  ((C.val.val[v]).filterMap id).toList
-
-theorem incident_colors_of_colored_nbors (v : Vertex n) :
-  incidentColorsOn c n G C v =
-  (coloredNbors c n G C v).val.filterMap (fun x => color c n G C (v, x)) := by
-  unfold incidentColorsOn coloredNbors color
-  simp_all [List.filterMap_filter]
-  split; rename_i _ _ C h1 h2 _ _
-  simp_all [List.filterMap_filter, Option.isSome_iff_ne_none]
-  have : C[v].toList = List.map (fun x ↦ C[v][x]'(by simp_all)) (List.finRange n) := by
-    ext1 i
-    simp [Option.map]; split
-    all_goals rename_i _ j hj
-    · apply Array.getElem?_eq_some_iff.mpr
-      rcases (List.getElem?_eq_some_iff.mp hj) with ⟨k, _⟩
-      have : (List.finRange n).length = n := by exact List.length_finRange
-      rw [List.length_finRange] at k
-      simp_all; congr
-      rename_i h; rw [← h]
-    · apply Array.getElem?_eq_none_iff.mpr
-      have := List.getElem?_eq_none_iff.mp hj
-      rw [List.length_finRange] at this
-      specialize h2 C[v] (by exact Array.mem_of_getElem rfl)
-      simp_all
-  simp_all; congr
-  funext x
-  split_ifs
-  · assumption
-  · split; rfl
-
-theorem colored_nbors_subset_nbors (v : Vertex n) :
-  (coloredNbors c n G C v).val ⊆ (nbhd n G v).val := by
-  simp [coloredNbors]
-  split
-  case _ _ C _ _ h _ =>
-  intro x h'
-  simp_all
-  specialize h (v, x) h'
-  simp [present] at h
-  exact h.right
-
-theorem nodup_subset_eq_length_le {α : Type} [DecidableEq α] (L M : List α)
-  (hl : L.Nodup) (hm : M.Nodup) (hsubset : L ⊆ M) : L.length ≤ M.length := by
-  rw [← List.toFinset_card_of_nodup hl, ← List.toFinset_card_of_nodup hm]
-  apply Finset.card_le_card
-  repeat any_goals rw [← List.toFinset_eq]
-  repeat assumption
-
-theorem nodup_exists_mem_notMem_of_len_lt {α : Type} [DecidableEq α] (L M : List α)
-  (hl : L.Nodup) (hm : M.Nodup) (hlen : L.length < M.length) :
-  ∃ x ∈ M, x ∉ L := by
-  rw [← List.toFinset_card_of_nodup hl, ← List.toFinset_card_of_nodup hm] at hlen
-  apply Finset.exists_mem_notMem_of_card_lt_card at hlen
-  simp_all
-
-theorem colored_nbhd_size_le (v : Vertex n) :
-  (coloredNbors c n G C v).val.length ≤ degree n G v := by
-  let N := coloredNbors c n G C v
-  let X := nbhd n G v
-  simp [degree]
-  apply nodup_subset_eq_length_le
-  · exact N.prop.right
-  · exact X.prop.right
-  · exact colored_nbors_subset_nbors c n G C v
-
-def default : EdgeColoring c n G :=
-  have ⟨⟨X, h1⟩, ⟨h2, h3⟩⟩ := G
-  let C : Array (Array (Color c)) :=
-    Array.replicate X.size (Array.replicate X.size none)
-  have ax1 : coloringSizeAx c n C := by
-    unfold coloringSizeAx C
-    simp_all
-    constructor
-    any_goals intro _
-    all_goals exact h1
-  have ax2 : coloringRepresentsEdgesAx c n ⟨C, ax1⟩ ⟨⟨X, h1⟩, ⟨h2, h3⟩⟩ := by
-    simp [coloringRepresentsEdgesAx]
-    intro a b h
-    simp [C] at h
-  have ax3 : coloringValidAx c n ⟨C, ax1⟩ := by
-    simp [coloringValidAx, C]
-  have ax4 : coloringSymmAx c n ⟨C, ax1⟩ := by
-    simp [coloringSymmAx, C]
-    split; simp_all
-    rename_i _ _ _ _ h; subst h
-    simp
-  ⟨⟨C, ax1⟩, ⟨ax2, ax3, ax4⟩⟩
+variable (n : Nat) (c : Nat) (G : Graph n) (C : EdgeColoring n c G)
 
 /-
-
-def coloringValidAx (C : Mat c n) :=
-  have aux : ∀ v : Vertex n, v < C.val.size := by
-    intro v
-    linarith [v.isLt, C.prop.left]
-  ∀ v : Vertex n, (List.filterMap id (C.val[v]'(aux v)).toList).Nodup
-
-
+-- Can't be a color we already used!
+-- (we don't need to specify any other edge invariants,
+   because we know the edge is present in the graph)
 -/
 
 def edgeColorValid (e : Edge n) (a : Color c) : Prop :=
-  have ⟨_, _⟩ := edgesInRange c n G C e
-  have ⟨⟨C, ⟨_, _⟩⟩, ⟨_, _⟩⟩ := C
-  a ∉ C[e.1] ∧ a ∉ C[e.2]
+  a.isSome →
+  Array.count a
+  (C.val[e.1]'(by rw [C.sizeAx1]; exact e.1.isLt)) = 0 ∧
+  Array.count a
+  (C.val[e.2]'(by rw [C.sizeAx1]; exact e.2.isLt)) = 0
 
+variable
+  (e : Edge n) (a : Color c)
+
+def setEdge :=
+  let h := set_set_preserves_size n C.val C.sizeAx1 C.sizeAx2 a e.1 e.2
+  set_set n (set_set n C.val C.sizeAx1 C.sizeAx2 a e.1 e.2)
+    (by exact h.left) (by exact h.right) a e.2 e.1
+
+theorem edge_not_self_loop (hpres : present n G e) : e.1 ≠ e.2 := by
+  have := G.prop.right
+  contrapose! this
+  simp [graphNoSelfLoopsAx]
+  simp [present, nbhd] at hpres
+  rcases hpres with ⟨l, r⟩
+  simp_all
+  use e.2
+
+theorem setEdge_symm (hpres : present n G e) :
+  setEdge n c G C e a = setEdge n c G C (e.2, e.1) a := by
+  simp [setEdge]
+  apply set_set_comm
+  right
+  exact edge_not_self_loop n G e hpres
+
+theorem setEdge_sizeAx1 : (setEdge n c G C e a).size = n := by
+  have h := set_set_preserves_size n C.val C.sizeAx1 C.sizeAx2 a e.1 e.2
+  exact (set_set_preserves_size n (set_set n C.val C.sizeAx1 C.sizeAx2 a e.1 e.2)
+    (by exact h.left) (by exact h.right) a e.2 e.1).left
+
+theorem setEdge_sizeAx2 : ∀ i : Vertex n,
+  ((setEdge n c G C e a)[i]'(by
+    rw [setEdge_sizeAx1]; exact i.isLt)).size = n := by
+  have h := set_set_preserves_size n C.val C.sizeAx1 C.sizeAx2 a e.1 e.2
+  exact (set_set_preserves_size n (set_set n C.val C.sizeAx1 C.sizeAx2 a e.1 e.2)
+    (by exact h.left) (by exact h.right) a e.2 e.1).right
+
+theorem setEdge_spec1 (hpres : present n G e) :
+  ((setEdge n c G C e a)[e.1.val]'(by
+    rw [setEdge_sizeAx1]; exact e.1.isLt))[e.2.val]'(by
+    rw [← Fin.getElem_fin, setEdge_sizeAx2]; exact e.2.isLt) = a := by
+    have hsize := set_set_preserves_size n C.val C.sizeAx1 C.sizeAx2 a e.1 e.2
+    have h1 := set_set_spec2 n C.val C.sizeAx1 C.sizeAx2 a e.1 e.2 e.1 e.2 (by tauto)
+    have h2 := set_set_spec1 n (set_set n C.val C.sizeAx1 C.sizeAx2 a e.1 e.2)
+      hsize.left hsize.right a e.2 e.1 e.1 e.2 (by right; exact edge_not_self_loop n G e hpres)
+    rw [h1] at h2
+    exact Eq.symm h2
+
+theorem setEdge_spec2 :
+  ((setEdge n c G C e a)[e.2.val]'(by
+    rw [setEdge_sizeAx1]; exact e.2.isLt))[e.1.val]'(by
+    rw [← Fin.getElem_fin, setEdge_sizeAx2]; exact e.1.isLt) = a := by
+    have hsize := set_set_preserves_size n C.val C.sizeAx1 C.sizeAx2 a e.1 e.2
+    have h2 := set_set_spec2 n (set_set n C.val C.sizeAx1 C.sizeAx2 a e.1 e.2)
+      hsize.left hsize.right a e.2 e.1 e.2 e.1 (by tauto)
+    simp [setEdge]
+    exact h2
+
+theorem setEdge_spec3 : ∀ u v : Vertex n,
+  (e.1 ≠ u ∨ e.2 ≠ v) ∧ (e.2 ≠ u ∨ e.1 ≠ v) →
+  (C.val[u.val]'(by
+    rw [C.sizeAx1]; exact u.isLt))[v.val]'(by
+    rw [← Fin.getElem_fin, C.sizeAx2]; exact v.isLt) =
+    ((setEdge n c G C e a)[u.val]'(by
+    rw [setEdge_sizeAx1]; exact u.isLt))[v.val]'(by
+    rw [← Fin.getElem_fin, setEdge_sizeAx2]; exact v.isLt) := by
+    intro u v h
+    have hsize := set_set_preserves_size n C.val C.sizeAx1 C.sizeAx2 a e.1 e.2
+    have h1 := set_set_spec1 n C.val C.sizeAx1 C.sizeAx2 a e.1 e.2 u v (by tauto)
+    have h2 := set_set_spec1 n (set_set n C.val C.sizeAx1 C.sizeAx2 a e.1 e.2)
+      hsize.left hsize.right a e.2 e.1 u v (by tauto)
+    rwa [← h1] at h2
+
+theorem setEdge_spec4 : ∀ u : Vertex n,
+  (e.1 ≠ u ∧ e.2 ≠ u) →
+  C.val[u.val]'(by
+    rw [C.sizeAx1]; exact u.isLt) =
+    (setEdge n c G C e a)[u.val]'(by
+    rw [setEdge_sizeAx1]; exact u.isLt) := by
+    intro u h
+    have hsize := set_set_preserves_size n C.val C.sizeAx1 C.sizeAx2 a e.1 e.2
+    have h1 := set_set_spec3 n C.val C.sizeAx1 C.sizeAx2 a e.1 e.2 u (by tauto)
+    have h2 := set_set_spec3 n (set_set n C.val C.sizeAx1 C.sizeAx2 a e.1 e.2)
+      hsize.left hsize.right a e.2 e.1 u (by tauto)
+    rwa [← h1] at h2
+
+theorem setEdge_spec5 (hpres : present n G e) :
+  ∀ b : Color c,
+    Array.count b ((setEdge n c G C e a)[e.1.val]'(by rw [setEdge_sizeAx1]; exact e.1.isLt)) =
+    Array.count b (C.val[e.1.val]'(by rw [C.sizeAx1]; exact e.1.isLt)) -
+    (if (C.val[e.1.val]'(by rw [C.sizeAx1]; exact e.1.isLt))[e.2.val]'(by
+      rw [← Fin.getElem_fin, C.sizeAx2 e.1]; exact e.2.isLt) = b then 1 else 0) +
+    (if a = b then 1 else 0) := by
+    intro b
+    have hsize := set_set_preserves_size n C.val C.sizeAx1 C.sizeAx2 a e.1 e.2
+    have h1 := count_set_set n C.val C.sizeAx1 C.sizeAx2 a b e.1 e.2
+    have h2 := count_set_set' n (set_set n C.val C.sizeAx1 C.sizeAx2 a e.1 e.2)
+      hsize.left hsize.right a b e.2 e.1 (by exact Ne.symm (edge_not_self_loop n G e hpres))
+    have h3 := set_set_spec2 n C.val C.sizeAx1 C.sizeAx2 a e.1 e.2 e.1 e.2 (by tauto)
+    rw [h1] at h2
+    simp [setEdge, Fin.getElem_fin] at ⊢ h2
+    exact h2
+
+theorem setEdge_representsEdgesAx (hpres : present n G e) : ∀ f : Edge n,
+    (((setEdge n c G C e a)[f.1]'(by
+    rw [setEdge_sizeAx1]; exact f.1.isLt))[f.2]'(by
+    rw [setEdge_sizeAx2]; exact f.2.isLt)).isSome → present n G f := by
+  have hpres_symm : present n G (e.2, e.1) := by
+    exact ⟨hpres.right, hpres.left⟩
+  intro f hf
+  by_cases h : (f = e) ∨ (f = (e.2, e.1))
+  · rcases h with h | h
+    all_goals rwa [h]
+  · simp_rw [Prod.eq_iff_fst_eq_snd_eq] at h
+    push_neg at h
+    have aux := setEdge_spec3 n c G C e a f.1 f.2 (by tauto)
+    simp only [Fin.getElem_fin, ← aux] at hf
+    exact C.representsEdgesAx f hf
+
+theorem setEdge_validAx (hpres : present n G e) (hvalid : edgeColorValid n c G C e a) :
+  ∀ u v : Vertex n,
+    (((setEdge n c G C e a)[u]'(by
+      rw [setEdge_sizeAx1]; exact u.isLt))[v]'(by
+      rw [setEdge_sizeAx2]; exact v.isLt)).isSome →
+    Array.count (((setEdge n c G C e a)[u]'(by
+      rw [setEdge_sizeAx1]; exact u.isLt))[v]'(by
+      rw [setEdge_sizeAx2]; exact v.isLt))
+      ((setEdge n c G C e a)[u]'(by
+      rw [setEdge_sizeAx1]; exact u.isLt))
+      = 1 := by
+  intro u v huv
+  have := edge_not_self_loop n G e hpres
+  by_cases h : e.1 ≠ u ∧ e.2 ≠ u
+  · have h1 := setEdge_spec3 n c G C e a u v (by tauto)
+    have h2 := setEdge_spec4 n c G C e a u h
+    simp_rw [Fin.getElem_fin, ← h1, ← h2] at ⊢ huv
+    exact C.validAx u v huv
+  · push_neg at h
+    have spec1 := setEdge_spec1 n c G C e a hpres
+    have spec2 := setEdge_spec2 n c G C e a
+    wlog hu : e.1 = u generalizing e
+    specialize this (e.2, e.1)
+    have symm := setEdge_symm n c G C (e.2, e.1) a (And.comm.mp hpres)
+    simp at symm
+    simp [symm] at this
+    apply this
+    · exact And.comm.mp (hpres)
+    · simp [edgeColorValid] at hvalid ⊢
+      intro h
+      exact And.comm.mp (hvalid h)
+    any_goals simp_all
+    (expose_names; exact fun a ↦ hu_1 (id (Eq.symm a)))
+    simp_rw [← hu] at *
+    by_cases hv : e.2 = v
+    · rw [← hv] at ⊢ huv
+      simp_rw [spec1] at ⊢ huv
+      simp_rw [setEdge_spec5 n c G C e a hpres a, ← Fin.getElem_fin, (hvalid huv).left]
+      simp only [Fin.getElem_fin, zero_tsub, ↓reduceIte, zero_add]
+    · have aux1 := setEdge_spec3 n c G C e a e.1 v (by tauto)
+      have aux2 := setEdge_spec5 n c G C e a hpres ((C.val[e.1]'(by
+        rw [C.sizeAx1]; exact e.1.isLt))[v]'(by
+        rw [C.sizeAx2]; exact v.isLt))
+      simp_rw [← aux1] at huv
+      have aux3 := C.validAx e.1 v huv
+      simp_rw [Fin.getElem_fin] at *
+      simp_rw [← aux1, aux2]
+      rw [aux3]
+      split_ifs with h1 h2
+      any_goals ring_nf
+      · have aux4 := count_gt_one_if (C.val[e.1]'(by rw [C.sizeAx1]; exact e.1.isLt)) n
+          (by exact C.sizeAx2 e.1) v e.2 (by
+            constructor; exact fun a ↦ hv (Eq.symm a); exact beq_iff_eq.mpr (Eq.symm h1))
+        simp_rw [Fin.getElem_fin] at aux4
+        apply ne_of_gt at aux4
+        simp_all
+      · rename_i h2
+        rw [← h2] at aux3 huv
+        obtain ⟨hl, _⟩ := hvalid huv
+        apply Array.not_mem_of_count_eq_zero at hl
+        rw [h2] at hl
+        contrapose! hl
+        simp
+
+theorem setEdge_symmAx (hpres : present n G e) : ∀ u v : Vertex n,
+    (((setEdge n c G C e a)[u]'(by
+      rw [setEdge_sizeAx1]; exact u.isLt))[v]'(by
+      rw [setEdge_sizeAx2]; exact v.isLt)) =
+    (((setEdge n c G C e a)[v]'(by
+      rw [setEdge_sizeAx1]; exact v.isLt))[u]'(by
+      rw [setEdge_sizeAx2]; exact u.isLt)) := by
+  intro u v
+  by_cases h : (e.1 ≠ u ∨ e.2 ≠ v) ∧ (e.2 ≠ u ∨ e.1 ≠ v)
+  · have h1 := setEdge_spec3 n c G C e a u v h
+    have h2 := setEdge_spec3 n c G C e a v u (by tauto)
+    simp_rw [Fin.getElem_fin, ← h1, ← h2]
+    exact C.symmAx u v
+  · push_neg at h
+    rcases h with (⟨hl, hr⟩ | ⟨hl, hr⟩)
+    all_goals
+    have h1 := setEdge_spec1 n c G C e a hpres
+    have h2 := setEdge_spec2 n c G C e a
+    simp_rw [← hl, ← hr, Fin.getElem_fin, h1, h2]
 
 def setEdgeColor (e : Edge n) (a : Color c)
-  (h : present n G e) (h' : edgeColorValid c n G C e a) : EdgeColoring c n G :=
-  have ⟨h1, h2⟩ := edgesInRange c n G C e
-  have ⟨⟨C, ⟨ax1, ax2⟩⟩, ⟨ax3, ax4⟩⟩ := C
-  let C' := C.set e.1 <| C[e.1].set e.2 a
-  have aux1 : coloringSizeAx c n C' := by
-    unfold coloringSizeAx C' at *
-    constructor
-    · simp_all only [Fin.getElem_fin, Array.size_set]
-    · intro x h
-      have := Array.mem_or_eq_of_mem_set h
-      rcases this with this | this
-      all_goals simp_all only [Fin.getElem_fin, Array.size_set, Array.getElem_mem]
-  have aux2 : coloringRepresentsEdgesAx c n ⟨C', aux1⟩ G := by
-    unfold coloringRepresentsEdgesAx at *
-    simp; simp at ax3
-    intro u v h3
-    by_cases huv : e.1 = u ∧ e.2 = v
-    · rcases huv with ⟨hl, hr⟩
-      rw [← hl, ← hr]
-      exact h
-    apply ax3 u v
-    simp [C'] at h3; simp at huv
-    by_cases hu : e.1 = u
-    · have := @Array.getElem_set_ne _ C[u] e.2 (by simp_all) a v (by simp_all)
-      specialize this (by exact Fin.val_ne_of_ne (huv hu))
-      simp_all
-    · have := @Array.getElem_set_ne _ C e.1 h1 (C[e.1].set e.2 a) u (by simp_all)
-      specialize this (by exact Fin.val_ne_of_ne hu)
-      simp_all
-  have aux3 : coloringValidAx c n ⟨C', aux1⟩ := by
-    simp [coloringValidAx, C']
-    sorry
-  ⟨⟨C', aux1⟩, ⟨aux2, aux3⟩⟩
+  (hpres : present n G e) (hvalid : edgeColorValid n c G C e a) : EdgeColoring n c G where
+  val := setEdge n c G C e a
+  sizeAx1 := setEdge_sizeAx1 n c G C e a
+  sizeAx2 := setEdge_sizeAx2 n c G C e a
+  representsEdgesAx := setEdge_representsEdgesAx n c G C e a hpres
+  validAx := setEdge_validAx n c G C e a hpres hvalid
+  symmAx := setEdge_symmAx n c G C e a hpres
 
 def allColors : List (Fin c) := List.finRange c
 
 def freeColorsOn (v : Vertex n) :=
-  (allColors c).filter (fun x => x ∉ incidentColorsOn c n G C v)
+  (allColors c).filter (fun x => x ∉ incidentColorsOn n c G C v)
 
 theorem existsFreeColor (h : ↑(maxDegree n G) < c) :
-  ∀ v : Vertex n, (freeColorsOn c n G C v) ≠ [] := by
+  ∀ v : Vertex n, (freeColorsOn n c G C v) ≠ [] := by
   intro v
   simp [freeColorsOn]
   apply nodup_exists_mem_notMem_of_len_lt
-  simp [incidentColorsOn]
-  · exact (C.prop.right.left) v
+  · apply List.nodup_iff_count_le_one.mpr
+    simp [incidentColorsOn, List.count_filterMap]
+    have := C.validAx v
+    simp_all
+    intro a
+    by_cases h : (some a) ∈ C.val[v]'(by rw [C.sizeAx1]; exact v.isLt)
+    · apply le_iff_lt_or_eq.mpr
+      right
+      apply Array.getElem_of_mem at h
+      rcases h with ⟨i, hi1, hi2⟩
+      specialize this ⟨i, (by rw [C.sizeAx2] at hi1; exact hi1)⟩
+      simp_rw [Fin.getElem_fin, hi2] at *
+      simp [Array.count_eq_countP] at this
+      rw [← this]
+    · apply Array.count_eq_zero_of_not_mem at h
+      simp only [Fin.getElem_fin, Array.count_eq_countP] at h
+      rw [h]
+      linarith
   · simp [allColors]
     exact List.nodup_finRange c
   · simp [incident_colors_of_colored_nbors, allColors, List.length_finRange]
-    have hle : (coloredNbors c n G C v).val.length < c := by
-      have h1 := colored_nbhd_size_le c n G C v
+    have hle : (coloredNbors n c G C v).val.length < c := by
+      have h1 := colored_nbhd_size_le n c G C v
       have h2 := maxDegree_spec n G v
       exact lt_of_le_of_lt (le_trans h1 h2) h
     have hlt := List.length_filterMap_le
-      (fun x ↦ color c n G C (v, x)) ↑(coloredNbors c n G C v)
+      (fun x ↦ color n c G C (v, x)) ↑(coloredNbors n c G C v)
     exact Nat.lt_of_le_of_lt hlt hle
-
-
-/-
-
-No self edges
-
-
--/
-
-#exit
-
-variable (c : Nat) (n : Nat) (G : Graph n)
-  (nonempty : 0 < c)
-  (graphsize : G.size = n)
-  (edgeSet_symm : ∀ u v : Vertex n, (u, v) ∈ (edgeSet n G graphsize) ↔ v ∈ nbors n G graphsize u ∧ u ∈ nbors n G graphsize v)
-  (nbors_symm : ∀ u v : Vertex n, v ∈ nbors n G graphsize u ↔ u ∈ nbors n G graphsize v)
-
--- We choose 0 as the default value, to represent an uncolored edge
-
-abbrev Color := Fin (c + 1)
-abbrev EdgeColoring := Array (Array (Color c))
-
-variable
-  (C : EdgeColoring c)
-  (edgecoloring1 : C.size = n ∧ ∀ x ∈ C, x.size = n)
-
-include edgecoloring1
-
-theorem cx' (v : Vertex n) : v < C.size := by
-  rw [(edgecoloring1).left]
-  exact v.isLt
-
--- Accessing the color of an edge is always in bound
-theorem cx (e : Edge n) : e.1 < C.size ∧
-  e.2 < (C[e.1]'(cx' c n C edgecoloring1 e.1)).size := by
-  constructor
-  · exact cx' c n C edgecoloring1 e.1
-  · rw [(edgecoloring1).right]
-    · exact e.2.isLt
-    · exact Array.mem_of_getElem rfl
-
-def color (e : Edge n) :=
-  have := cx c n C edgecoloring1 e
-  C[e.1][e.2]
-
-def coloring_valid (C : EdgeColoring c) (h : C.size = n ∧ ∀ x ∈ C, x.size = n) :=
-  ∀ v : Vertex n, ((C[v]'(cx' c n C h v)).filter (fun c => c ≠ 0)).size ≤ degree n G graphsize v
-
-def default : EdgeColoring c :=
-  mkArray G.size (mkArray G.size 0)
-
-omit edgecoloring1 in
-include graphsize in
-theorem default_spec :
-  (default c n G).size = n ∧ ∀ x ∈ (default c n G), x.size = n := by
-  simp only [default, Array.size_mkArray, Array.mem_mkArray, ne_eq, List.length_eq_zero,
-    Array.toList_eq_nil_iff, and_imp, forall_eq_apply_imp_iff]
-  constructor
-  exact graphsize
-  intro h; exact graphsize
-
-omit edgecoloring1 in
-theorem default_spec' : coloring_valid c n G graphsize
-  (default c n G) (default_spec c n G graphsize) := by
-  simp [coloring_valid, default]
-
-def allColors : List (Color c) :=
-  let L := List.finRange (c + 1)
-  have : 0 < c + 1 := by
-    exact Nat.add_pos_left nonempty 1
-  L.erase ⟨0, this⟩
-
-variable
-  (edgecoloring2 : coloring_valid c n G graphsize C edgecoloring1)
-  (edgecoloring3 : ∀ u v, u ∉ nbors n G graphsize v → color c n G C edgecoloring1 (u, v) = 0)
-
-def setEdgeColor (e : Edge n) (a : Color c) : EdgeColoring c :=
-  let e' := (e.2, e.1)
-  have := cx c n C edgecoloring1 e
-  let C' := C.set e.1 <| C[e.1].set e.2 a
-  have h1 : C'.size = n := by
-    simp only [Fin.getElem_fin, Array.size_set, C']; exact edgecoloring1.left
-  have h2 : ∀ x ∈ C', x.size = n := by
-    simp only [Fin.getElem_fin, C']
-    intro x hx
-    have := Array.mem_or_eq_of_mem_set hx
-    rcases this with l | r
-    exact edgecoloring1.right x l
-    simp only [r, Array.size_set, Array.getElem_mem, edgecoloring1, C']
-  have := cx c n C' ⟨h1, h2⟩ e'
-  C'.set e'.1 <| C'[e'.1].set e'.2 a
-
-example (x : α) (A : Array α) (i : Nat) (h : i < A.size) :
-  x = A[i] → x ∈ A := by
-  exact fun a ↦ Array.mem_of_getElem (id (Eq.symm a))
-
-theorem setEdgeColor_spec (e : Edge n) (a : Color c) :
-  (setEdgeColor c n G C edgecoloring1 e a).size = n ∧
-  ∀ x ∈ (setEdgeColor c n G C edgecoloring1 e a), x.size = n := by
-  simp only [setEdgeColor, Fin.getElem_fin, Array.size_set]
-  constructor
-  exact edgecoloring1.left
-  intro x hx
-  have := Array.mem_or_eq_of_mem_set hx
-  rcases this with this | this
-  · have := Array.mem_or_eq_of_mem_set this
-    rcases this with l | r
-    exact edgecoloring1.right x l
-    simp only [r, Array.size_set, Array.getElem_mem, edgecoloring1]
-  · have aux := cx c n C edgecoloring1 e
-    have h1 : ((Array.set C (↑e.fst) (C[↑e.fst].set (↑e.snd) a))).size = n := by
-      simp only [Fin.getElem_fin, Array.size_set, edgecoloring1]
-    have h2 : ∀ x ∈ ((Array.set C (↑e.fst) (C[↑e.fst].set (↑e.snd) a))), x.size = n := by
-      intro x hx
-      have := Array.mem_or_eq_of_mem_set hx
-      rcases this with l | r
-      exact edgecoloring1.right x l
-      simp [r, Array.size_set, Array.getElem_mem]
-      have : C[↑e.fst] ∈ C := by
-        exact Array.mem_of_getElem rfl
-      exact edgecoloring1.right C[↑e.fst] this
-    have h3 : ((Array.set C (↑e.fst) (C[↑e.fst].set (↑e.snd) a)))[↑e.snd].size = n := by
-      simp_all only [Fin.is_lt, Fin.getElem_fin, Array.getElem_mem]
-    have h4 := Array.size_set ((Array.set C (↑e.fst) (C[↑e.fst].set (↑e.snd) a))[↑e.snd])
-    simp only [h3] at h4
-    simp_all only [Fin.is_lt, Fin.getElem_fin, Array.size_set, Array.getElem_mem, implies_true]
-
-include edgecoloring3 in
-theorem aux (e : Edge n) (a : Color c) (h : e ∈ edgeSet n G graphsize) :
-  ∀ u v, u ∉ nbors n G graphsize v → color c n G (setEdgeColor c n G C edgecoloring1 e a)
-  (setEdgeColor_spec c n G C edgecoloring1 e a) (u, v) = 0 := by
-  intro u v h2
-  specialize edgecoloring3 u v h2
-  simp [setEdgeColor, color] at *
-  let C' := setEdgeColor c n G C edgecoloring1 e a
-  have h' := setEdgeColor_spec c n G C edgecoloring1 e a
-  have aux := cx' c n C' h'
-  have : ∀ v, v ≠ e.1 ∧ v ≠ e.2 → C[v] = C'[v]'(aux v) := by
-    intro v h
-    simp [C', setEdgeColor]
-    repeat rw [Array.getElem_set_ne]
-    all_goals apply Fin.val_ne_of_ne; apply Ne.symm
-    exact h.left
-    exact h.right
-  rw [← edgecoloring3]
-  have : ∀ f : Edge n, f.1 ≠ e.1 ∧ f.1 ≠ e.2 → color c n G C edgecoloring1 f = color c n G C' h' f := by
-    intro f hf
-    simp [color, C', setEdgeColor]
-    have aux := this f.1 hf
-    simp [C', setEdgeColor] at aux
-    simp [aux]
-  simp [color, C', setEdgeColor] at this
-  specialize this u v
-  apply Eq.symm
-  apply this
-  sorry
-  sorry
-
-def setEdgeColor_spec' (e : Edge n) (a : Color c) (h : e ∈ edgeSet n G graphsize) :
-  coloring_valid c n G graphsize (setEdgeColor c n G C edgecoloring1 e a)
-  (setEdgeColor_spec c n G C edgecoloring1 e a) := by
-  let C' := setEdgeColor c n G C edgecoloring1 e a
-  have h' := setEdgeColor_spec c n G C edgecoloring1 e a
-  have aux := cx' c n C' h'
-  have : ∀ v, v ≠ e.1 ∧ v ≠ e.2 → C[v] = C'[v]'(aux v) := by
-    intro v h
-    simp [C', setEdgeColor]
-    repeat rw [Array.getElem_set_ne]
-    all_goals apply Fin.val_ne_of_ne; apply Ne.symm
-    exact h.left
-    exact h.right
-  unfold coloring_valid degree at *
-  intro v
-  by_cases h : v ≠ e.1 ∧ v ≠ e.2
-  · specialize this v h
-    unfold C' at this
-    rw [← this]
-    exact edgecoloring2 v
-  · by_cases h2 : v = e.1
-    dsimp -zeta [setEdgeColor]
-    rw [h2]
-    repeat rw [Array.getElem_set_self]
-    simp only
-    sorry
-    sorry
-    sorry
-
-def getIncidentColors (v : Vertex n) : List (Color c) :=
-  (nbors n G graphsize v).map (fun a => color c n G C edgecoloring1 (v, a))
-
-def getNborWithColor? (v : Vertex n) (a : Color c) : Option (Vertex n) :=
-  let choices := (nbors n G graphsize v).filter (fun x => color c n G C edgecoloring1 (v, x) = a)
-  match choices with
-  | [] => none
-  | u :: _ => some u
-
-def getFreeColors (v : Vertex n) : List (Color c) :=
-  let incident := getIncidentColors c n G graphsize C edgecoloring1 v
-  (allColors c nonempty).filter (fun x => x ∉ incident)
-
-def freeOn (a : Color c) (v : Vertex n) :=
-  a ∈ getFreeColors c n G nonempty graphsize C edgecoloring1 v
-
-def incidentOn (a : Color c) (v : Vertex n) :=
-  a ∈ getIncidentColors c n G graphsize C edgecoloring1 v
-
-include edgecoloring2 in
-theorem existsFreeColor (h : maxDegree n G graphsize < c) :
-  ∀ v, getFreeColors c n G nonempty graphsize C edgecoloring1 v ≠ [] := by
-  intro v hv
-  have h1 : C[v].size = n := by
-    apply edgecoloring1.right
-    exact Array.mem_of_getElem rfl
-  simp [*, getFreeColors, getIncidentColors, allColors, color, nbors] at hv
-  let X := (List.finRange (c + 1)).erase 0
-  let Y := (C[v].filter (fun a => a ≠ 0))
-  have h2 : ∀ a ∈ X, a ∈ C[v] := by
-    intro a ha
-    have := hv a ha
-    rcases this with ⟨x, hx1, hx2⟩
-    exact Array.mem_of_getElem hx2
-  have h3 : ∀ a ∈ X, a ∈ Y := by
-    intro a ha
-    have aux1 := h2 a ha
-    simp only [X, List.finRange, List.ofFn_succ, List.erase_cons_head, List.mem_ofFn,
-      Fin.exists_succ_eq, ne_eq] at ha
-    simp only [Y, Fin.getElem_fin, ne_eq, decide_not, id_eq, Int.reduceNeg, Array.mem_filter,
-      Bool.not_eq_eq_eq_not, Bool.not_true, decide_eq_false_iff_not]
-    exact ⟨aux1, ha⟩
-  have h4 : X.length = c := by
-    simp only [X, List.mem_finRange, List.length_erase_of_mem, List.length_finRange,
-      add_tsub_cancel_right]
-  have h5 : Y.size ≥ c := by
-    have aux1 : X ⊆ Y.toList := by
-      simp [List.subset_def]
-      intro a ha
-      exact h3 a ha
-    have aux2 : X.Nodup := by
-      simp [X, List.finRange, List.Nodup]
-      intro i j hij
-      exact Fin.ne_of_lt hij
-    have aux3 : X.toFinset.card = X.length := by
-      have : (List.finRange (c+1)).erase 0 = ((List.finRange (c+1)).erase 0).dedup := by
-        exact Eq.symm (List.Nodup.dedup aux2)
-      simp [List.toFinset, Multiset.toFinset, X, List.finRange, List.ofFn, this]
-    have aux4 : Y.toList.toFinset.card ≤ Y.toList.length := by
-      exact List.toFinset_card_le Y.toList
-    simp [← h4]
-    have aux5 : X.toFinset ⊆ Y.toList.toFinset := by
-      simp [Finset.subset_def]
-      have : X = X.dedup := by exact Eq.symm (List.Nodup.dedup aux2)
-      rw [← this]
-      have : Y.toList ⊆ Y.toList.dedup := by exact List.subset_dedup Y.toList
-      exact fun _ x ↦ this (aux1 x)
-    have aux6 : X.toFinset.card ≤ Y.toList.toFinset.card := by
-      exact Finset.card_le_card aux5
-    rw [aux3] at aux6
-    exact Nat.le_trans aux6 aux4
-  specialize edgecoloring2 v
-  have := maxDegree_spec n G graphsize v
-  have : degree n G graphsize v < c := by linarith
-  have : Y.size < c := by
-    exact lt_of_le_of_lt edgecoloring2 this
-  linarith
-
-end EdgeColoring
