Vizing/new/Nbhd.lean
@@ -1,0 +1,134 @@
+import Vizing.new.Graph
+import Mathlib.Data.List.Lemmas
+import Mathlib.Data.Finset.Card
+import Vizing.new.Upstream
+
+set_option linter.dupNamespace false
+
+namespace Nbhd
+open Graph
+
+/-
+Defining some useful lemmas about colored neighborhoods,
+and the notion of a valid edge coloring,
+where `EdgeColoring c` represents a c-edge-coloring of a graph on [n] vertices.
+-/
+
+variable (n : Nat) (c : Nat) (G : Graph n)
+abbrev Color := Option (Fin c)
+
+instance : DecidableEq (Color c) := by
+  infer_instance
+
+structure EdgeColoring where
+  val : Array (Array (Color c))
+  sizeAx1 : val.size = n
+  sizeAx2 : ∀ i : Fin n, val[i].size = n
+  representsEdgesAx : ∀ e : Edge n,
+    ((val[e.1]'(by
+    rw [sizeAx1]; exact e.1.isLt))[e.2]'(by
+    rw [sizeAx2]; exact e.2.isLt)).isSome → present n G e
+  validAx :
+    ∀ u v : Vertex n,
+    ((val[u]'(by rw [sizeAx1]; exact u.isLt))[v]'(by rw [sizeAx2]; exact v.isLt)).isSome →
+    @Array.count (Color c) _
+    ((val[u]'(by rw [sizeAx1]; exact u.isLt))[v]'(by rw [sizeAx2]; exact v.isLt))
+    (val[u]'(by rw [sizeAx1]; exact u.isLt)) = 1
+  symmAx :
+    ∀ u v : Vertex n,
+    ((val[u]'(by rw [sizeAx1]; exact u.isLt))[v]'(by rw [sizeAx2]; exact v.isLt)) =
+    ((val[v]'(by rw [sizeAx1]; exact v.isLt))[u]'(by rw [sizeAx2]; exact u.isLt))
+deriving DecidableEq
+
+variable (C : EdgeColoring n c G)
+
+def color (e : Edge n) :=
+  (C.val[e.1]'(by rw [C.sizeAx1]; exact e.1.isLt))[e.2]'
+  (by rw [C.sizeAx2]; exact e.2.isLt)
+
+def coloredNbors (v : Vertex n) : Nbors n :=
+  have := G.prop.right
+  let NV := (C.val[v]'(by rw [C.sizeAx1]; exact v.isLt))
+  have aux2 : NV.size = n := by
+    exact C.sizeAx2 v
+  have aux3 : ∀ x : Vertex n, x < NV.size := by
+    simp_all
+  let N := (List.finRange n).filter (fun x => (NV[x]'(aux3 x)).isSome)
+  have ax1 : nborsSizeAx n N := by
+    have h4: v ∉ N := by
+      have := C.representsEdgesAx (v, v)
+      have this' := G.prop.right v
+      simp_all [N, present, nbhd]
+      exact this
+    have h5 : N.length ≤ (List.finRange n).length := by
+      apply List.length_filter_le
+    rcases lt_or_eq_of_le h5 with (h5 | h5)
+    · simp_all; assumption
+    · unfold N at h4 h5
+      apply List.length_filter_eq_length_iff.mp at h5
+      specialize h5 v (by exact List.mem_finRange v)
+      simp_all
+  have ax2 : nborsRepeatsAx n N := by
+    apply List.Nodup.filter
+    exact List.nodup_finRange n
+  ⟨N, ⟨ax1, ax2⟩⟩
+
+def incidentColorsOn (v : Vertex n) :=
+  ((C.val[v]'(by rw [C.sizeAx1]; exact v.isLt)).filterMap id).toList
+
+theorem nbhd_to_indexed_nbhd (v : Vertex n) (A : Array (Array (Color c)))
+  (h1 : A.size = n) (h2 : ∀ i : Fin n, A[i].size = n) :
+  A[v].toList = List.map (fun x ↦ A[v][x]'(by simp_all)) (List.finRange n) := by
+  ext1 i
+  simp [Option.map]; split
+  all_goals rename_i j hj
+  · apply Array.getElem?_eq_some_iff.mpr
+    rcases (List.getElem?_eq_some_iff.mp hj) with ⟨h3, h4⟩
+    have : i < A[v].size := by
+      rw [h2]
+      rwa [List.length_finRange] at h3
+    use this
+    congr
+    simp at h4
+    exact Fin.mk.inj_iff.mp h4
+  · apply Array.getElem?_eq_none_iff.mpr
+    have := List.getElem?_eq_none_iff.mp hj
+    rw [List.length_finRange] at this
+    simp_all
+
+theorem incident_colors_of_colored_nbors (v : Vertex n) :
+  incidentColorsOn n c G C v =
+  (coloredNbors n c G C v).val.filterMap (fun x => color n c G C (v, x)) := by
+  unfold incidentColorsOn coloredNbors color
+  simp_all [List.filterMap_filter]
+  simp_all [List.filterMap_filter, Option.isSome_iff_ne_none]
+  have := nbhd_to_indexed_nbhd n c v C.val C.sizeAx1 C.sizeAx2
+  simp_all; congr
+  funext x
+  split_ifs
+  · assumption
+  · rfl
+
+theorem colored_nbors_subset_nbors (v : Vertex n) :
+  (coloredNbors n c G C v).val ⊆ (nbhd n G v).val := by
+  simp [coloredNbors]
+  intro x h'
+  have := C.representsEdgesAx (v, x)
+  simp_all [present]
+
+theorem colored_nbhd_size_le (v : Vertex n) :
+  (coloredNbors n c G C v).val.length ≤ degree n G v := by
+  let N := coloredNbors n c G C v
+  let X := nbhd n G v
+  simp [degree]
+  apply nodup_subset_eq_length_le
+  · exact N.prop.right
+  · exact colored_nbors_subset_nbors n c G C v
+
+def default : EdgeColoring n c G where
+  val := Array.replicate n (Array.replicate n none)
+  sizeAx1 := by simp only [Array.size_replicate]
+  sizeAx2 := by simp
+  representsEdgesAx := by simp
+  validAx := by simp
+  symmAx := by simp
